day1/checker.fsti
@@ -6,6 +6,8 @@ open Ast
 val size       : #a:Type -> term a -> nat
 val closed     : #a:Type -> nat -> e:term a -> Tot bool (decreases (size e))
 
+val toClosed   : #a:Type -> e:term a -> Tot (result (t:(term a){closed 0 t}))
+
 val typeInfer  : n:nat -> context -> e:(term infer){closed n e} -> Tot (result typeL) (decreases (size e))
 val typeCheck  : n:nat -> context -> e:(term check){closed n e} -> t:typeL -> Tot (result unit) (decreases %[size e;t])
 val typeInfer0 : context -> e:(term infer){closed 0 e} -> result typeL
